theories/FOL/Util/Semantics.v
@@ -2,181 +2,205 @@
 
 Require Export Undecidability.FOL.Util.FOL_facts.
 Import ListAutomationNotations.
+Require Import Vector.
+
 Local Set Implicit Arguments.
+Local Unset Strict Implicit.
 
-(** ** Variables and Substitutions *)
+(*** Full Syntax ***)
 
-Fixpoint vars_t (t : term) : list var :=
-  match t with
-  | V v => [v]
-  | P p => []
-  | t_f b t => vars_t t
-  | t_e => []
-  end.
+Inductive full_logic_binop : Type :=
+(*| Conj : full_logic_binop
+| Disj : full_logic_binop*)
+| Impl : full_logic_binop.
 
-Fixpoint consts_t (t : term) : list var :=
-  match t with
-  | V v => []
-  | P p => [p]
-  | t_f b t => consts_t t
-  | t_e => []
-  end.
+Inductive full_logic_quant : Type :=
+| All : full_logic_quant
+(*| Ex : full_logic_quant*).
 
-Fixpoint subst_t x y (t : term) : term :=
-  match t with
-  | V v => if Dec (v = x) then y else V v
-  | P p => P p
-  | t_e => t_e
-  | t_f b t => t_f b (subst_t x y t)
-  end.
+Instance full_operators : operators :=
+{| binop := full_logic_binop ; quantop := full_logic_quant |}.
 
-Fixpoint consts {b} (phi : form b) : list var :=
-  match phi with
-  | Pr t1 t2  => consts_t t1 ++ consts_t t2
-  | Fal
-  | Q => []
-  | Impl phi psi => consts phi ++ consts psi
-  | All v phi => v :: consts phi
-  end.
+Notation "∀ Phi" := (quant All Phi) (at level 50).
+(*Notation "∃ Phi" := (quant Ex Phi) (at level 50).
+Notation "A ∧ B" := (bin Conj A B) (at level 41).
+Notation "A ∨ B" := (bin Disj A B) (at level 42).*)
+Notation "A '-->' B" := (bin Impl A B) (at level 43, right associativity).
 
-Fixpoint subst {b} x t phi :=
-  match phi with
-  | Pr t1 t2 => Pr (subst_t x t t1) (subst_t x t t2)
-  | Q => Q
-  | Fal => Fal
-  | Impl phi1 phi2 => Impl (subst x t phi1) (subst x t phi2)
-  | All v phi => All v (if Dec (x = v) then phi else subst x t phi)
-  end.
+Section fixb.
 
-Definition consts_l {b} A := flat_map (@consts b) A.
-Definition fresh (y : var) A := ~ y el A.
-
-
-Fixpoint mkfresh (l : list nat) :=
-  match l with
-  | [] => 0
-  | x :: l => S x + mkfresh l
-  end.
-
-Lemma mkfresh_spec l a : a el l -> a < mkfresh l.
-Proof.
-  induction l.
-  - firstorder.
-  - cbn; intros [ | ]; firstorder lia.
-Qed.
-
-Lemma make_fresh A : {z | fresh z A}.
-Proof.
-  exists (mkfresh A). intros ? % mkfresh_spec. lia.
-Defined.
-
-Lemma app_sub X (A A' B B' : list X) :
-  A <<= A' -> B <<= B' -> A ++ B <<= A' ++ B'.
-Proof.
-  intros H1 H2 x [H|H] % in_app_iff.
-  all: apply in_app_iff; auto.
-Qed.
-
-
-(** ** Interpretations *)
-
-Class interp (domain : Type) (rho : nat -> domain) :=
-  {
-    i_f : bool -> domain -> domain ;
-    i_e : domain ;
-    i_P : domain -> domain -> Prop ;
-    i_Q : Prop
-  }.
-
-Section Semantics.
-
-  Notation const := nat.
-  Variable domain : Type.  
-
-  Definition env := var -> domain.
-
-  Variable (eta : env).
-  Context {I : interp eta}.
+  Context {Σ_funcs : funcs_signature}.
+  Context {Σ_preds : preds_signature}.
+  Context {ff : falsity_flag}.
   
-  Fixpoint eval (rho : env) (t : term) : domain :=
-    match t with
-    | V s => rho s
-    | P p => eta p
-    | t_f b t => i_f b (eval rho t)
-    | t_e => i_e
+  Fixpoint impl (A : list form) phi :=
+    match A with
+    | [] => phi
+    | psi :: A => bin Impl psi (impl A phi)
     end.
-  
-  Definition update {X} (rho : var -> X) (v : var) (d : X) :=
-    (fun v' => if (Dec (v = v')) then d else rho v').
-  
-  Notation "rho [[ v := d ]]" := (update rho v d) (at level 20).
-  
-  Fixpoint sat {b} (rho : env) (phi : form b) : Prop :=
-    match phi with
-    | Pr t1 t2 =>  i_P (eval rho t1) (eval rho t2)
-    | Q => i_Q
-    | Fal => False
-    | Impl phi psi => sat rho phi -> sat rho psi
-    | All v phi => forall d : domain, sat (rho [[ v := d ]]) phi
-    end.
-  Notation "rho ⊫ A" := (forall psi, psi el A -> sat rho psi) (at level 20).
+
+End fixb.
+
+
+
+(*** Tarski Semantics ***)
+
+Section Tarski.
+
+  Context {Σ_funcs : funcs_signature}.
+  Context {Σ_preds : preds_signature}.
+
+  (** Semantic notions *)
+
+  Section Semantics.
+
+    Variable domain : Type.
+
+    Class interp := B_I
+      {
+        i_f : forall f : syms, vec domain (ar_syms f) -> domain ;
+        i_P : forall P : preds, vec domain (ar_preds P) -> Prop ;
+      }.
+
+    Definition env := nat -> domain.
+
+    Context {I : interp}.
+
+    Fixpoint eval (rho : env) (t : term) : domain :=
+      match t with
+      | var s => rho s
+      | func f v => i_f (Vector.map (eval rho) v)
+      end.
+
+    Fixpoint sat {ff : falsity_flag} (rho : env) (phi : form) : Prop :=
+      match phi with
+      | atom P v => i_P (Vector.map (eval rho) v)
+      | falsity => False
+      | bin Impl phi psi => sat rho phi -> sat rho psi
+      (*| bin Conj phi psi => sat rho phi /\ sat rho psi
+      | bin Disj phi psi => sat rho phi \/ sat rho psi
+      | quant Ex phi => exists d : domain, sat (d .: rho) phi*)
+      | quant All phi => forall d : domain, sat (d .: rho) phi
+      end.
+
+  End Semantics.
+
   Notation "rho ⊨ phi" := (sat rho phi) (at level 20).
-
-  Context {b : logic}.
   
-  Lemma impl_sat A rho phi :
-    sat rho (A ==> phi) <-> ((forall psi, psi el A -> sat rho psi) -> sat rho phi).
-  Proof.
-    induction A; cbn; firstorder congruence.
-  Qed.
+  Section Substs.
+    
+    Variable D : Type.
+    Variable I : interp D.
+        
+    Lemma eval_ext rho xi t :
+      (forall x, rho x = xi x) -> eval rho t = eval xi t.
+    Proof.
+      intros H. induction t; cbn.
+      - now apply H.
+      - f_equal. apply map_ext_in. now apply IH.
+    Qed.
 
-  Lemma impl_sat' A rho phi :
-    sat rho (A ==> phi) -> ((forall psi, psi el A -> sat rho psi) -> sat rho phi).
-  Proof.
-    eapply impl_sat.
-  Qed. 
-  
-End Semantics.
+    Lemma eval_comp rho xi t :
+      eval rho (subst_term xi t) = eval (xi >> eval rho) t.
+    Proof.
+      induction t; cbn.
+      - reflexivity.
+      - f_equal. rewrite map_map. apply map_ext_in, IH.
+    Qed.
 
-Tactic Notation "destruct" "_":=
-  match goal with
-  | [ |- context[match ?X with _ => _ end] ] => destruct X
-  | [ H : context[match ?X with _ => _ end] |- _ ] => destruct X 
-  end.
-Ltac decs :=
-  unfold update; repeat destruct _;
-  subst; cbn; try congruence; try reflexivity; auto.
+    Lemma sat_ext {ff : falsity_flag} rho xi phi :
+      (forall x, rho x = xi x) -> rho ⊨ phi <-> xi ⊨ phi.
+    Proof.
+      induction phi in rho, xi |- *; cbn; intros H.
+      - reflexivity.
+      - erewrite map_ext; try reflexivity. intros t. now apply eval_ext.
+      - specialize (IHphi1 rho xi). specialize (IHphi2 rho xi). destruct b0; intuition.
+      - destruct q.
+        + split; intros H' d; eapply IHphi; try apply (H' d). 1,2: intros []; cbn; intuition.
+        (* + split; intros [d H']; exists d; eapply IHphi; try apply H'. all: intros []; cbn; intuition.*)
+    Qed.
 
-Notation "rho [[ v := d ]]" := (update rho v d) (at level 20).
+    Lemma sat_ext' {ff : falsity_flag} rho xi phi :
+      (forall x, rho x = xi x) -> rho ⊨ phi -> xi ⊨ phi.
+    Proof.
+      intros Hext H. rewrite sat_ext. exact H.
+      intros x. now rewrite (Hext x).
+    Qed.
 
-Arguments sat {_ _} _ {_} _ _, {_} _ _ {_} _ _.
-Arguments interp {_} _, _ _.
+    Lemma sat_comp {ff : falsity_flag} rho xi phi :
+      rho ⊨ (subst_form xi phi) <-> (xi >> eval rho) ⊨ phi.
+    Proof.
+      induction phi in rho, xi |- *; cbn.
+      - reflexivity.
+      - erewrite map_map, map_ext; try reflexivity. intros t. apply eval_comp.
+      - specialize (IHphi1 rho xi). specialize (IHphi2 rho xi). destruct b0; intuition.
+      - destruct q.
+        + setoid_rewrite IHphi. split; intros H d; eapply sat_ext. 2, 4: apply (H d).
+          all: intros []; cbn; trivial; now setoid_rewrite eval_comp.
+        (* + setoid_rewrite IHphi. split; intros [d H]; exists d; eapply sat_ext. 2, 4: apply H.
+          all: intros []; cbn; trivial; now setoid_rewrite eval_comp.*)
+    Qed.
+
+    Lemma sat_subst {ff : falsity_flag} rho sigma phi :
+      (forall x, eval rho (sigma x) = rho x) -> rho ⊨ phi <-> rho ⊨ (subst_form sigma phi).
+    Proof.
+      intros H. rewrite sat_comp. apply sat_ext. intros x. now rewrite <- H.
+    Qed.
+
+    Lemma sat_single {ff : falsity_flag} (rho : nat -> D) (Phi : form) (t : term) :
+      (eval rho t .: rho) ⊨ Phi <-> rho ⊨ subst_form (t..) Phi.
+    Proof.
+      rewrite sat_comp. apply sat_ext. now intros [].
+    Qed.
+
+    
+  End Substs.
+
+End Tarski.
+
+Arguments sat {_ _ _ _ _} _ _, {_ _ _} _ {_} _ _.
+Arguments interp {_ _} _, _ _ _.
 
 
 
 Notation "p ⊫ A" := (forall psi, psi el A -> sat _ p psi) (at level 20).
 Notation "p ⊨ phi" := (sat _ p phi) (at level 20).
 
-Implicit Type b : logic.
+Section Defs.
 
-Definition valid b phi := forall D eta (I : interp D eta) rho, rho ⊨ phi.
-Definition valid_L b A := forall D eta (I : interp D eta) rho, rho ⊫ A.
-Definition satis b phi := exists D eta (I : interp D eta) rho, rho ⊨ phi.
-Definition fullsatis b A := exists D eta (I : interp D eta) rho, rho ⊫ A.
+  Context {Σ_funcs : funcs_signature}.
+  Context {Σ_preds : preds_signature}.
+  Context {ff : falsity_flag}.
 
+  Definition valid phi := forall D (I : interp D) rho, rho ⊨ phi.
+  Definition valid_L A := forall D (I : interp D) rho, rho ⊫ A.
+  Definition satis phi := exists D (I : interp D) rho, rho ⊨ phi.
+  Definition fullsatis A := exists D (I : interp D) rho, rho ⊫ A.
+
+End Defs.
 
 
 (** Trivial Model *)
 
 Section TM.
 
-  Instance TM : interp unit (fun _ => tt) :=
-    {| i_f := fun _ _ => tt; i_e := tt; i_P := fun _ _ => True; i_Q := True |}.
+  Context {Σ_funcs : funcs_signature}.
+  Context {Σ_preds : preds_signature}.
 
-  Fact TM_sat (rho : var -> unit) (phi : form frag) :
+  Instance TM : interp unit :=
+    {| i_f := fun _ _ => tt; i_P := fun _ _ => True; |}.
+
+  Fact TM_sat (rho : nat -> unit) (phi : form falsity_off) :
     sat TM rho phi.
   Proof.
-    revert rho. induction phi using form_frag_ind; cbn; auto.
+    revert rho. remember falsity_off as ff. induction phi; cbn; trivial.
+    - discriminate.
+    - destruct b0; auto.
+    - destruct q; firstorder.
   Qed.
 
 End TM.
+
+
+
+
